refactor(library/init/meta): avoid '_core' idiom using default parameters
I kept a few core methods (e.g., exact_core and apply_core). Reason:
if we use default parameters

    meta constant exact (e : expr) (md := semireducible) : tactic unit

then, we will not be able to write

    to_expr p >>= exact

The workaround is

    do t <- to_expr p, exact t

or
    to_expr p >>= (fun x, exact x)

One alternative is to change how we handle default parameters, and
eta-expand applications that involve default parameters.
We may also have an attribute [eta_expand]. Then

    attribute [eta_expand] foo

instructs the elaborator to automatically eta-expand foo-applications.
The attribute would give users more control, and avoid potential
performance problems. Without the attribute, then for every function
application the elaborator has to check the type and decide whether it
must be eta-expanded or not.

@gebner @kha What do you think?

src/frontends/lean/token_table.cpp
@@ -108,7 +108,7 @@ void init_token_table(token_table & t) {
          "import", "inductive", "structure", "class", "universe", "universes", "local",
          "precedence", "reserve", "infixl", "infixr", "infix", "postfix", "prefix", "notation",
          "exit", "set_option", "open", "export", "override", "@[",
-         "attribute", "persistent", "instance", "include", "omit", "init_quotient",
+         "attribute", "instance", "include", "omit", "init_quotient",
          "init_hits", "declare_trace", "run_command", "add_key_equivalence",
          "#compile", "#unify", nullptr};
 
