src/library/tactic/cases_tactic.cpp
@@ -485,7 +485,7 @@ cases(environment const & env, options const & opts, transparency_mode const & m
     return r;
 }
 
-vm_obj tactic_cases_core(vm_obj const & m, vm_obj const & H, vm_obj const & ns, vm_obj const & _s) {
+vm_obj tactic_cases_core(vm_obj const & H, vm_obj const & ns, vm_obj const & m, vm_obj const & _s) {
     tactic_state const & s   = to_tactic_state(_s);
     try {
         if (!s.goals()) return mk_no_goals_exception(s);
