tests/lean/run/1295.lean
@@ -3,10 +3,10 @@ open tactic
 
 example : true := by do
 a ← to_expr `((0 : ℕ)), b ← to_expr `(nat.zero),
-fail_if_success (unify_core transparency.none a b),
+fail_if_success (unify a b transparency.none),
 triv
 
 example (x : ℕ) : true := by do
 a ← to_expr `((x + 0 : ℕ)), b ← to_expr `(x + nat.zero),
-fail_if_success (unify_core transparency.none a b),
+fail_if_success (unify a b transparency.none),
 triv
