tests/lean/run/cases_bug2.lean
@@ -1,4 +1,4 @@
 open tactic
 
 example (a : nat) : 0 = nat.succ a → false
-:= by intro1 >>= cases
+:= by do h ← intro1, cases h
