tests/lean/run/induction_tac3.lean
@@ -3,7 +3,7 @@ open tactic
 example (p q : Prop) : p ∨ q → q ∨ p :=
 by do
   H ← intro `H,
-  induction_core semireducible H `or.rec [],
+  induction H `or.rec [],
   constructor_idx 2, assumption,
   constructor_idx 1, assumption
 
@@ -11,7 +11,7 @@ open nat
 example (n : ℕ) : n = 0 ∨ n = succ (pred n) :=
 by do
   n ← get_local `n,
-  induction_core semireducible n `nat.rec [],
+  induction n `nat.rec [],
   constructor_idx 1, reflexivity,
   constructor_idx 2, reflexivity,
   return ()
@@ -19,6 +19,6 @@ by do
 example (n : ℕ) (H : n ≠ 0) : n > 0 → n = succ (pred n) :=
 by do
   n ← get_local `n,
-  induction_core semireducible n `nat.rec [],
+  induction n `nat.rec [],
   intro `H1, contradiction,
   intros, reflexivity
