tests/lean/run/induction_tactic_delta.lean
@@ -11,5 +11,5 @@ definition foo'.rec := @foo.rec
 
 example : Pi (x : foo'), x = x :=
 by do x ← intro `x,
-      induction_core reducible x `foo'.rec [],
+      induction x `foo'.rec [],
       reflexivity
