tests/lean/run/meta_tac4.lean
@@ -14,8 +14,8 @@ by do
     unify h1 h2,
     unify h2 h3,
     unify h1 h3,
-    (unify_core reducible h1 h2 <|> trace "H1 =?= H2 failed if only reducible constants can be unfolded"),
-    unify_core reducible h2 h3,
-    (unify_core reducible h1 h3 <|> trace "H1 =?= H3 failed if only reducible constants can be unfolded"),
+    (unify h1 h2 reducible <|> trace "H1 =?= H2 failed if only reducible constants can be unfolded"),
+    unify h2 h3 reducible,
+    (unify h1 h3 reducible <|> trace "H1 =?= H3 failed if only reducible constants can be unfolded"),
     assumption,
     return ()
